libcrux-iot/ml-kem/proofs/fstar/extraction/Libcrux_iot_ml_kem.Constants.fst
@@ -3,6 +3,9 @@ module Libcrux_iot_ml_kem.Constants
 open FStar.Mul
 open Core_models
 
+/// Each field element needs floor(log_2(FIELD_MODULUS)) + 1 = 12 bits to represent
+let v_BITS_PER_COEFFICIENT: usize = mk_usize 12
+
 /// Coefficients per ring element
 let v_COEFFICIENTS_IN_RING_ELEMENT: usize = mk_usize 256
 
@@ -16,6 +19,9 @@ let v_BYTES_PER_RING_ELEMENT: usize = v_BITS_PER_RING_ELEMENT /! mk_usize 8
 let v_SHARED_SECRET_SIZE: usize = mk_usize 32
 
 let v_CPA_PKE_KEY_GENERATION_SEED_SIZE: usize = mk_usize 32
+
+/// SHA3 256 digest size
+let v_H_DIGEST_SIZE: usize = mk_usize 32
 
 /// K * BITS_PER_RING_ELEMENT / 8
 /// [eurydice] Note that we can\'t use const generics here because that breaks
